dataplane/Timely_Infrastructure.thy
@@ -616,11 +616,11 @@ abbreviation init_conf where
   "init_conf summary cgs \<equiv> the (propagate_all summary (init_c_pts summary cgs))"
 
 record ('p, 'd, 'd1, 't) operator_state_ty = "('p, 'd, 't) operator_state" +
-  en1 :: "'d1 \<Rightarrow> 'd" de1 :: "'d \<Rightarrow> 'd1"
+  en1 :: "'d1 \<Rightarrow> 'd" de1 :: "'d \<Rightarrow> 'd1" is_en1 :: "'d \<Rightarrow> bool"
 record ('p, 'd, 'd1, 'd2, 't) operator_state_ty2 = "('p, 'd, 'd1, 't) operator_state_ty" +
-  en2 :: "'d2 \<Rightarrow> 'd" de2 :: "'d \<Rightarrow> 'd2"
+  en2 :: "'d2 \<Rightarrow> 'd" de2 :: "'d \<Rightarrow> 'd2" is_en2 :: "'d \<Rightarrow> bool"
 record ('p, 'd, 'd1, 'd2, 'd3, 't) operator_state_ty3 = "('p, 'd, 'd1, 'd2, 't) operator_state_ty2" +
-  en3 :: "'d3 \<Rightarrow> 'd" de3 :: "'d \<Rightarrow> 'd3"
+  en3 :: "'d3 \<Rightarrow> 'd" de3 :: "'d \<Rightarrow> 'd3" is_en3 :: "'d \<Rightarrow> bool"
 
 definition "graph_to_edges summary = (\<lambda> l1. [l2 \<leftarrow> Enum.enum. \<not> is_empty_antichain (summary l1 l2) \<and> is_Src (port l1) \<and> is_Trg (port l2) ])"
 
